pulse/lib/pulse/core/PulseCore.BaseHeapSig.fsti
@@ -1,0 +1,98 @@
+module PulseCore.BaseHeapSig
+open PulseCore.HeapSig
+open FStar.Ghost
+open FStar.PCM
+module H = PulseCore.Heap
+val base_heap : heap_sig u#a
+val core_ghost_ref_as_addr (_:core_ghost_ref) : GTot nat
+val select_ghost (i:nat) (m:base_heap.sep.core) : GTot (option (H.cell u#a))
+val ghost_ctr (b:base_heap.mem) : GTot nat
+
+val interp_ghost_pts_to 
+      (i:core_ghost_ref)
+      (#meta:bool)
+      (#a:Type u#a)
+      (#pcm:FStar.PCM.pcm a)
+      (v:a)
+      (h0:(base_heap u#a).mem)
+: Lemma
+  (requires interpret (base_heap.ghost_pts_to meta #a #pcm i v) h0)
+  (ensures (
+    match select_ghost (core_ghost_ref_as_addr i) (base_heap.sep.lens_core.get h0) with
+    | None -> False
+    | Some c ->
+      let H.Ref meta' a' pcm' v' = c in
+      meta == reveal meta' /\
+      a == a' /\
+      pcm == pcm' /\
+      compatible pcm v v'))
+      
+val ghost_pts_to_compatible_equiv 
+      (#meta:bool)
+      (#a:Type)
+      (#pcm:_)
+      (x:ghost_ref a pcm)
+      (v0:a)
+      (v1:a{composable pcm v0 v1})
+: Lemma ((base_heap.ghost_pts_to meta x v0 `base_heap.star` base_heap.ghost_pts_to meta x v1) ==
+         (base_heap.ghost_pts_to meta x (op pcm v0 v1)))
+
+val ghost_extend
+    (meta:erased bool)
+    (#ex:inames base_heap)
+    (#a:Type u#a)
+    (#pcm:pcm a)
+    (x:erased a{pcm.refine x})
+: ghost_action_except base_heap (ghost_ref a pcm) ex    
+      base_heap.emp 
+      (fun r -> base_heap.ghost_pts_to meta r x)
+
+val ghost_read
+    (#ex:inames base_heap)
+    (#meta:erased bool)
+    (#a:Type)
+    (#p:pcm a)
+    (r:ghost_ref a p)
+    (x:erased a)
+    (f:(v:a{compatible p x v}
+        -> GTot (y:a{compatible p y v /\
+                     FStar.PCM.frame_compatible p x v y})))
+: ghost_action_except base_heap (erased (v:a{compatible p x v /\ p.refine v})) ex
+    (base_heap.ghost_pts_to meta r x)
+    (fun v -> base_heap.ghost_pts_to meta r (f v))
+
+val ghost_write
+    (#ex:inames base_heap)
+    (#meta:erased bool)
+    (#a:Type)
+    (#p:pcm a)
+    (r:ghost_ref a p)
+    (x y:Ghost.erased a)
+    (f:FStar.PCM.frame_preserving_upd p x y)
+: ghost_action_except base_heap unit ex
+    (base_heap.ghost_pts_to meta r x)
+    (fun _ -> base_heap.ghost_pts_to meta r y)
+
+val ghost_share
+    (#ex:inames base_heap)
+    (#meta:erased bool)
+    (#a:Type)
+    (#pcm:pcm a)
+    (r:ghost_ref a pcm)
+    (v0:FStar.Ghost.erased a)
+    (v1:FStar.Ghost.erased a{composable pcm v0 v1})
+: ghost_action_except base_heap unit ex
+    (base_heap.ghost_pts_to meta r (v0 `op pcm` v1))
+    (fun _ -> base_heap.ghost_pts_to meta r v0 `base_heap.star` base_heap.ghost_pts_to meta r v1)
+
+val ghost_gather
+    (#ex:inames base_heap)
+    (#meta:erased bool)
+    (#a:Type)
+    (#pcm:pcm a)
+    (r:ghost_ref a pcm)
+    (v0:FStar.Ghost.erased a)
+    (v1:FStar.Ghost.erased a)
+: ghost_action_except base_heap (squash (composable pcm v0 v1)) ex
+    (base_heap.ghost_pts_to meta r v0 `base_heap.star` base_heap.ghost_pts_to meta r v1)
+    (fun _ -> base_heap.ghost_pts_to meta r (op pcm v0 v1))
